%% -- ln-part-d3_4 --%%
Since $b(v^{*},v^{*}) = 0$ we obtain $b(x,v^{*}) = 0$ for all $x \in M$ (Lemma 1.1.a), hence $T(xv) = S(x)v$.

\begin{enumerate}[(a)]
\item 
Since $s(|\phi|)M$ is a closed right ideal, the closed face $F := s(|\phi|)(M_{+})s(|\phi|)$ determines $s(|\phi|)M$ uniquely, i.e.,
%% --
\[
s(|\phi|)M = \{x \in M : xx^{*} \in F\}
\]
%% --
[Pedersen (1979), Theorem 1.5.2].
Since $T$ is a Schwarz map and $s(|\phi|)M$ is $T$-invariant, it follows $TF \subseteq F$.
On the other hand, if $x \in s(|\phi|)M$ then $xx^{*} \in F$.
Consequently,
%% --
\[
0 \leq S(x)S(x)^{*} \leq T(xx^{*}) \in F,
\]
%% --
whence $S(x) \in s(|\phi|)M$.

Next we show $T(u^{*}u) = u^{*}u$ and $Su^{*} = u^{*} \in s(|\phi|)M$.
First of all
%% --
\[
0 \leq (Su^{*} - u^{*})(Su^{*} - u^{*})^{*} \leq
\]
%% --
%% --
\[
\leq T(u^{*}u) - u^{*}S(u^{*})^{*} - (Su^{*})u + u^{*}u.
\]
%% --
Since $S_{*}\phi = \phi$, $T_{*}|\phi| = |\phi|$ and $\phi = u|\phi|$ it follows
%% --
\[
0 \leq |\phi|((Su^{*} - u^{*})(Su^{*} - u^{*})^{*}) \leq
\]
%% --
%% --
\[
\leq 2|\phi|(u^{*}u) - |\phi|(S(u^{*})u)^{*} - |\phi|(S(u^{*})u) =
\]
%% --
%% --
\[
= 2|\phi|(uu^{*}) - \phi(u^{*})^{*} - \phi(u^{*}) =
\]
%% --
%% --
\[
= 2(|\phi|(u^{*}u) - |\phi|(u^{*}u)) = 0.
\]
%% --

Since $(Su^{*} - u^{*})(Su^{*} - u^{*}) \in F$ and $|\phi|$ is faithful on $F$ we obtain $Su^{*} = u^{*}$.
Consequently,
%% --
\[
0 \leq u^{*}u = (Su^{*})(Su^{*})^{*} \leq T(u^{*}u).
\]
%% --

Hence $T(u^{*}u) = u^{*}u$ by the faithfulness and $T$-invariance of $|\phi|$.
\end{enumerate}